All equivaleces in Propositional Loigc carries over to Predicate logic.

Prove $(\forall x.A \land B) \leftrightarrow ((\forall x.A) \land (\forall x.B))$

$$\huge\frac{\frac{\frac{\frac{\frac{\frac{}{\forall x.A \land B}1}{A \land B}[\forall E]}{A}[\land E]}{\forall x.A}[\forall I]\, \, \, \frac{\frac{\frac{\frac{}{\forall x.A \land B}1}{A \land B}[\forall E]}{B}[\land E]}{\forall x.B}[\forall I]}{(\forall x.A) \land (\forall x.B)}[\land I]}{(\forall x.A \land B) \rightarrow (\forall x.A) \land (\forall x.B)}1[-> I]$$

